chapter03

exercises/chapter03-state-machines/exercise02.dfy
@@ -13,17 +13,21 @@
 
 // Define all the relevant state in this datatype.
 // FIXME: fill in here (solution: 8 lines)
- datatype Variables = Variables(tableSize: nat)
+ datatype Variables = Variables(tableSize: nat, leftChopstick: seq<bool>, rightChopstick: seq<bool>)
  {
    ghost predicate WellFormed() {
      && 0 < tableSize
+     && |leftChopstick| == |rightChopstick| == tableSize
+     && forall i | 0 <= i < tableSize :: !(rightChopstick[i] && leftChopstick[(i+1) % tableSize])
    }
  }
 // END EDIT
 
 ghost predicate Init(v:Variables) {
   // FIXME: fill in here (solution: 3 lines)
-      true  // Replace me
+  && v.tableSize > 0
+  && |v.leftChopstick| == |v.rightChopstick| == v.tableSize
+  && forall i | 0 <= i < v.tableSize :: v.leftChopstick[i] == v.rightChopstick[i] == false
   // END EDIT
 }
 
@@ -34,33 +38,47 @@ ghost predicate Init(v:Variables) {
 // Philosopher with index philosopherIndex acquires left chopstick
 ghost predicate AcquireLeft(v:Variables, v':Variables, philosopherIndex:nat) {
   // FIXME: fill in here (solution: 5 lines)
-      true  // Replace me
+  && v.WellFormed()
+  && v'.WellFormed()
+  && philosopherIndex < v.tableSize
+  && v' == v.(leftChopstick := v.leftChopstick[philosopherIndex := true])
   // END EDIT
 }
 
 // Philosopher with index philosopherIndex acquires right chopstick
 ghost predicate AcquireRight(v:Variables, v':Variables, philosopherIndex:nat) {
   // FIXME: fill in here (solution: 5 lines)
-      true  // Replace me
+  && v.WellFormed()
+  && v'.WellFormed()
+  && philosopherIndex < v.tableSize
+  && v' == v.(rightChopstick := v.rightChopstick[philosopherIndex := true])
   // END EDIT
 }
 
 // Philosopher with index philosopherIndex releases both chopsticks
 ghost predicate ReleaseBoth(v:Variables, v':Variables, philosopherIndex:nat) {
   // FIXME: fill in here (solution: 5 lines)
-      true  // Replace me
+  && v.WellFormed()
+  && v'.WellFormed()
+  && philosopherIndex < v.tableSize
+  && v' == v.(leftChopstick := v.leftChopstick[philosopherIndex := false],
+              rightChopstick := v.rightChopstick[philosopherIndex := false])
   // END EDIT
 }
 
 datatype Step =
     // FIXME: fill in here (solution: 3 lines)
-     Step()  // Replace me
+    | LeftStep(philosopherIndex: nat)
+    | RightStep(philosopherIndex: nat)
+    | ReleaseStep(philosopherIndex: nat)
     // END EDIT
 
 ghost predicate NextStep(v:Variables, v':Variables, step: Step) {
   match step
   // FIXME: fill in here (solution: 3 lines)
-   case Step => false  // Replace me
+   case LeftStep(philosopherIndex) => AcquireLeft(v, v', philosopherIndex)
+   case RightStep(philosopherIndex) => AcquireRight(v, v', philosopherIndex)
+   case ReleaseStep(philosopherIndex) => ReleaseBoth(v, v', philosopherIndex)
   // END EDIT
 }
 
@@ -81,7 +99,7 @@ ghost predicate NoSticksAcquired(v: Variables)
   requires v.WellFormed()
 {
   // FIXME: fill in here (solution: 8 lines)
-          true // Replace me
+  forall i | 0 <= i < v.tableSize :: v.leftChopstick[i] == v.rightChopstick[i] == false
   // END EDIT
 }
 
@@ -94,7 +112,7 @@ ghost predicate BothSticksAcquired(v: Variables, philosopherIndex: nat)
   requires v.WellFormed()
 {
   // FIXME: fill in here (solution: 6 lines)
-      true
+  v.leftChopstick[philosopherIndex] == v.rightChopstick[philosopherIndex] == true
   // END EDIT
 }
 
@@ -121,5 +139,14 @@ lemma PseudoLiveness(philosopherIndex:nat) returns (behavior:seq<Variables>)
   ensures BothSticksAcquired(behavior[|behavior|-1], philosopherIndex)  // Behavior ultimately achieves acquisition for philosopherIndex
 {
   // FIXME: fill in here (solution: 6 lines)
+  var v1 := Variables(tableSize := 3, leftChopstick := [false, false, false], rightChopstick := [false, false, false]);
+
+  var v2 := v1.(leftChopstick := v1.leftChopstick[philosopherIndex := true]);
+  assert NextStep(v1, v2, LeftStep(philosopherIndex));
+
+  var v3 := v2.(rightChopstick := v2.rightChopstick[philosopherIndex := true]);
+  assert NextStep(v2, v3, RightStep(philosopherIndex));
+
+  behavior := [v1, v2, v3];
   // END EDIT
 }
